Getting ANNOYED

coq/Network/PacketTotalOrder.v
@@ -2,138 +2,99 @@ Set Implicit Arguments.
 
 Require Import Coq.Structures.Equalities.
 Require Import NArith.BinNat.
-Require Import Word.WordInterface.
+Require Import Bag.TotalOrder.
+Require Import Word.WordTheory.
 Require Import Network.Packet.
 
 Local Open Scope list_scope.
 Local Open Scope N_scope.
 
 Axiom bytes_le : bytes -> bytes -> Prop.
+Axiom Instance TotalOrder_bytes : TotalOrder bytes_le.
 
+Definition proj_tcp r := 
+  match r with
+    | Tcp src dst seq ack off flags win chk urg payload =>
+      (src,dst,seq,ack,off,flags,win,chk,urg,payload)
+  end.
 
-Record tcp : Type := Tcp {
-  tcpSrc : tpPort;
-  tcpDst : tpPort;
-  tcpSeq : Word32.t;
-  tcpAck : Word32.t;
-  tcpOffset : Word8.t;
-  tcpFlags : Word16.t; (** nine lower bits *)
-  tcpWindow : Word16.t;
-  tcpChksum : Word8.t;
-  tcpUrgent : Word8.t;
-  tcpPayload : bytes
-}.
+Definition inj_tcp tup := 
+  match tup with
+    | (src,dst,seq,ack,off,flags,win,chk,urg,payload) =>
+      Tcp src dst seq ack off flags win chk urg payload
+  end.
 
-Record icmp : Type := Icmp {
-  icmpType : Word8.t;
-  icmpCode : Word8.t;
-  icmpChksum : Word16.t;
-  icmpPayload : bytes
-}.
+Local Notation "x ** y" := (PairOrdering x y) (at level 71, left associativity).
+Local Notation "x +++ y" := (SumOrdering x y) (at level 70, right associativity).
 
-Inductive tpPkt : nwProto -> Type :=
-  | TpTCP : tcp -> tpPkt Const_0x6
-  | TpICMP : icmp -> tpPkt Const_0x1
-  | TpUnparsable : forall (proto : nwProto), bytes -> tpPkt proto.
+Definition tcp_le :=
+  (Word16.le ** Word16.le ** Word32.le ** Word32.le ** Word8.le ** 
+     Word16.le ** Word16.le ** Word8.le ** Word8.le **  bytes_le).
 
-Record ip : Type := IP {
-  pktIPVhl : Word8.t;
-  pktIPTos : nwTos;
-  pktIPLen : Word16.t;
-  pktIPIdent : Word16.t;
-  pktIPFlags : Word8.t; (* 3 bits *)
-  pktIPFrag : Word16.t; (** 13 bits *)
-  pktIPTtl : Word8.t;
-  pktIPProto : nwProto;
-  pktIPChksum : Word16.t;
-  pktIPSrc :  nwAddr;
-  pktIPDst : nwAddr;
-  pktTpHeader : tpPkt pktIPProto
-}.
+Hint Resolve TotalOrder_sum TotalOrder_pair TotalOrder_bytes 
+  Word16.TotalOrder Word32.TotalOrder Word8.TotalOrder.
 
-Inductive arp : Type :=
-  | ARPQuery : dlAddr -> nwAddr -> nwAddr -> arp
-  | ARPReply : dlAddr -> nwAddr -> dlAddr -> nwAddr -> arp.
+Instance TotalOrder_tcp : TotalOrder (ProjectOrdering proj_tcp tcp_le).
+Proof.
+  apply TotalOrder_Project with (g:=inj_tcp).
+  + unfold tcp_le. auto 20.
+  + unfold inverse. destruct x; auto.
+Qed.
 
-Inductive nw : dlTyp -> Type :=
-  | NwIP : ip -> nw Const_0x800
-  | NwARP : arp -> nw Const_0x806
-  | NwUnparsable : forall (typ : dlTyp), bytes -> nw typ.
+Definition proj_icmp r :=
+  match r with
+    | Icmp typ code chksum payload => (typ, code, chksum, payload)
+  end.
 
-Record packet : Type := Packet {
-  pktDlSrc : dlAddr;
-  pktDlDst : dlAddr;
-  pktDlTyp : dlTyp;
-  pktDlVlan : dlVlan;
-  pktDlVlanPcp : dlVlanPcp;
-  pktNwHeader : nw pktDlTyp
-}.
+Definition inj_icmp tup :=
+  match tup with
+    | (typ, code, chksum, payload) => Icmp typ code chksum payload
+  end.
 
+Definition icmp_le := Word8.le ** Word8.le ** Word16.le ** bytes_le.
 
-Inductive tcp_le : tcp -> tcp -> Prop :=
-  | 
+Instance TotalOrder_icmp : TotalOrder (ProjectOrdering proj_icmp icmp_le).
+Proof.
+  apply TotalOrder_Project with (g:=inj_icmp).
+  + unfold icmp_le. auto 20.
+  + unfold inverse. destruct x; auto.
+Qed.
 
+Definition proj_tpPkt (proto : nwProto) (r : tpPkt proto) := 
+  match r with
+    | TpTCP tcp => inl (proj_tcp tcp)
+    | TpICMP icmp => inr (inl (proj_icmp icmp))
+    | TpUnparsable proto bytes => inr (inr (proto,bytes))
+  end.
 
-Axiom bytes : Type.
+Definition tcpTup :=
+  (Word16.Word.t * Word16.Word.t * Word32.Word.t * Word32.Word.t * Word8.Word.t * 
+   Word16.Word.t * Word16.Word.t * Word8.Word.t * Word8.Word.t *  bytes) %type.
 
-(* JNF: I wonder if we should extract this to something
-else. Cstruct.t has funny equalities due to the behavior of
-shift. Maybe just a string? *)
-Extract Constant bytes => "Cstruct.t".
+Definition icmpTup :=
+  (Word8.Word.t * Word8.Word.t * Word16.Word.t * bytes) %type.
 
-Section Constants.
+Definition inj_tpPkt tup := 
+  match tup in sum _ _ return
+        match tup with 
+          | inl _ => tpPkt Const_0x6 
+          | inr (inl _) => tpPkt Const_0x1
+          | inr (inr (proto, _)) => tpPkt proto
+        end with
+    | inl tcp => TpTCP (inj_tcp tcp)
+    | inr (inl icmp) => TpICMP (inj_icmp icmp)
+    | inr (inr (proto,bytes)) => TpUnparsable proto bytes
+  end.
+
+Definition tpPkt_le := tcp_le +++ icmp_le +++ (Word8.le ** bytes_le).
   
-  Definition Const_0x800 := @Word16.Mk 2048 eq_refl.
-  Definition Const_0x806 := @Word16.Mk 2054 eq_refl.
-  Definition Const_0x6 := @Word8.Mk 6 eq_refl.
-  Definition Const_0x7 := @Word8.Mk 7 eq_refl.
-  Definition Const_0x1 := @Word8.Mk 1 eq_refl.
 
-End Constants.
+(* This is getting stupid. Why are these dependent types? *)
+Instance TotalOrder_tpPkt `(proto : Word8.Word.t) : TotalOrder (ProjectOrdering (@proj_tpPkt proto) tpPkt_le).
+Proof.
+Abort.
 
-Extract Constant Const_0x800 => "0x800".
-Extract Constant Const_0x806 => "0x806".
-Extract Constant Const_0x6 => "0x6".
-Extract Constant Const_0x7 => "0x7".
-Extract Constant Const_0x1 => "0x1".
-
-Definition portId := Word16.t.
-Definition dlAddr := Word48.t.
-Definition dlTyp := Word16.t.
-Definition dlVlan := Word16.t.
-Definition dlVlanPcp := Word8.t. (* 3 bits *)
-Definition nwAddr := Word32.t.
-Definition nwProto := Word8.t.
-Definition nwTos := Word8.t. (** 6 bits *)
-Definition tpPort := Word16.t.
-
-Unset Elimination Schemes.
-
-Record tcp : Type := Tcp {
-  tcpSrc : tpPort;
-  tcpDst : tpPort;
-  tcpSeq : Word32.t;
-  tcpAck : Word32.t;
-  tcpOffset : Word8.t;
-  tcpFlags : Word16.t; (** nine lower bits *)
-  tcpWindow : Word16.t;
-  tcpChksum : Word8.t;
-  tcpUrgent : Word8.t;
-  tcpPayload : bytes
-}.
-
-Record icmp : Type := Icmp {
-  icmpType : Word8.t;
-  icmpCode : Word8.t;
-  icmpChksum : Word16.t;
-  icmpPayload : bytes
-}.
-
-Inductive tpPkt : nwProto -> Type :=
-  | TpTCP : tcp -> tpPkt Const_0x6
-  | TpICMP : icmp -> tpPkt Const_0x1
-  | TpUnparsable : forall (proto : nwProto), bytes -> tpPkt proto.
-
+(*
 Record ip : Type := IP {
   pktIPVhl : Word8.t;
   pktIPTos : nwTos;
@@ -166,202 +127,5 @@ Record packet : Type := Packet {
   pktDlVlanPcp : dlVlanPcp;
   pktNwHeader : nw pktDlTyp
 }.
-
-Section Accessors.
-  (** These accessors return zero if a field does not exist. *)
-
-  Definition pktNwSrc pk :=
-    match pk with
-      | {| pktNwHeader := hdr |} => 
-        match hdr with
-          | NwIP ip => pktIPSrc ip
-          | NwARP (ARPQuery _ ip _) => ip
-          | NwARP (ARPReply _ ip _ _) => ip
-          | NwUnparsable _ _ => Word32.zero
-        end
-    end.
-
-  Definition pktNwDst pk :=
-    match pk with
-      | {| pktNwHeader := hdr |} => 
-        match hdr with
-          | NwIP ip => pktIPDst ip
-          | NwARP (ARPQuery _ _ ip) => ip
-          | NwARP (ARPReply _ _ _ ip) => ip
-          | NwUnparsable _ _ => Word32.zero
-        end
-    end.
-
-  Definition pktNwProto pk :=
-    match pk with
-      | {| pktNwHeader := hdr |} => 
-        match hdr with
-          | NwIP ip => pktIPProto ip
-          | NwARP (ARPQuery _ _ _) => Word8.zero
-          | NwARP (ARPReply _ _ _ _) => Word8.zero
-          | NwUnparsable _ _ => Word8.zero
-        end
-    end.
-
-  Definition pktNwTos pk :=
-    match pk with
-      | {| pktNwHeader := hdr |} => 
-        match hdr with
-          | NwIP ip => pktIPTos ip
-          | NwARP (ARPQuery _ _ _) => Word8.zero
-          | NwARP (ARPReply _ _ _ _) => Word8.zero
-          | NwUnparsable _ _ => Word8.zero
-        end
-    end.
-
-  Definition pktTpSrc pk :=
-    match pk with
-      | {| pktNwHeader := hdr |} => 
-        match hdr with
-          | NwIP ip => 
-            match pktTpHeader ip with
-              | TpTCP frag => tcpSrc frag
-              | TpICMP _ => Word16.zero
-              | TpUnparsable _ _ => Word16.zero
-            end
-          | NwARP (ARPQuery _ _ _) => Word16.zero
-          | NwARP (ARPReply _ _ _ _) => Word16.zero
-          | NwUnparsable _ _ => Word16.zero
-        end
-    end.
-
-  Definition pktTpDst pk :=
-    match pk with
-      | {| pktNwHeader := hdr |} => 
-        match hdr with
-          | NwIP ip => 
-            match pktTpHeader ip with
-              | TpTCP frag => tcpDst frag
-              | TpICMP _ => Word16.zero
-              | TpUnparsable _ _ => Word16.zero
-            end
-          | NwARP (ARPQuery _ _ _) => Word16.zero
-          | NwARP (ARPReply _ _ _ _) => Word16.zero
-          | NwUnparsable _ _ => Word16.zero
-        end
-    end.
-
-End Accessors.
-
-Section Setters.
-  (** These fail silently if the field does not exist. *)
-
-  Definition setDlSrc pk dlSrc :=
-    match pk with
-      | Packet _ dlDst dlTyp dlVlan dlVlanPcp nw =>
-        @Packet dlSrc dlDst dlTyp dlVlan dlVlanPcp nw
-    end.
-
-  Definition setDlDst pk dlDst :=
-    match pk with
-      | Packet dlSrc _ dlTyp dlVlan dlVlanPcp nw =>
-        @Packet dlSrc dlDst dlTyp dlVlan dlVlanPcp nw
-    end.
-
-  Definition setDlVlan pk dlVlan :=
-    match pk with
-      | Packet dlSrc dlDst dlTyp _ dlVlanPcp nw =>
-        @Packet dlSrc dlDst dlTyp dlVlan dlVlanPcp nw
-    end.
-
-  Definition setDlVlanPcp pk dlVlanPcp :=
-    match pk with
-      | Packet dlSrc dlDst dlTyp dlVlan _ nw =>
-        @Packet dlSrc dlDst dlTyp dlVlan dlVlanPcp nw
-    end.
-
-  Definition nw_setNwSrc (typ : dlTyp) (nwPkt : nw typ) src : nw typ :=
-    match nwPkt in nw typ return nw typ with
-      | NwIP (IP vhl tos len ident flags frag ttl proto chksum _ dst tp) =>
-        NwIP (@IP vhl tos len ident flags frag ttl proto chksum src dst tp)
-      | NwARP arp => NwARP arp
-      | NwUnparsable typ b => NwUnparsable typ b
-    end.
-
-  Definition nw_setNwDst (typ : dlTyp)(nwPkt : nw typ) dst : nw typ :=
-    match nwPkt in nw typ return nw typ with
-      | NwIP (IP vhl tos len ident flags frag ttl proto chksum src _ tp) =>
-        NwIP (@IP vhl tos len ident flags frag ttl proto chksum src dst tp)
-      | NwARP arp => NwARP arp
-      | NwUnparsable typ b => NwUnparsable typ b
-    end.
-
-  Definition nw_setNwTos (typ : dlTyp) (nwPkt : nw typ) tos : nw typ :=
-    match nwPkt in nw typ return nw typ with
-      | NwIP (IP vhl _ len ident flags frag ttl proto chksum src dst tp) =>
-        NwIP (@IP vhl tos len ident flags frag ttl proto chksum src dst tp)
-      | NwARP arp => NwARP arp
-      | NwUnparsable typ b => NwUnparsable typ b
-    end.
-
-  Definition setNwSrc pk nwSrc :=
-    match pk with
-      | Packet dlSrc dlDst dlTyp dlVlan dlVlanPcp nw =>
-        @Packet dlSrc dlDst dlTyp dlVlan dlVlanPcp (nw_setNwSrc nw nwSrc)
-    end.
-
-  Definition setNwDst pk nwDst :=
-    match pk with
-      | Packet dlSrc dlDst dlTyp dlVlan dlVlanPcp nw =>
-        @Packet dlSrc dlDst dlTyp dlVlan dlVlanPcp (nw_setNwDst nw nwDst)
-    end.
-
-  Definition setNwTos pk nwTos :=
-    match pk with
-      | Packet dlSrc dlDst dlTyp dlVlan dlVlanPcp nw =>
-        @Packet dlSrc dlDst dlTyp dlVlan dlVlanPcp (nw_setNwTos nw nwTos)
-    end.
-
-  Definition tp_setTpSrc (proto : nwProto) (tp : tpPkt proto) src : tpPkt proto := 
-    match tp in (tpPkt proto) return (tpPkt proto) with
-      | TpTCP (Tcp _ dst seq ack off flags win chksum urgent payload) => 
-        TpTCP (Tcp src dst seq ack off flags win chksum urgent payload)
-      | TpICMP icmp => TpICMP icmp
-      | TpUnparsable proto payload => TpUnparsable proto payload
-    end.
-
-  Definition tp_setTpDst (proto : nwProto) (tp : tpPkt proto) dst : tpPkt proto := 
-    match tp in (tpPkt proto) return (tpPkt proto) with
-      | TpTCP (Tcp src _ seq ack off flags win chksum urgent payload) => 
-        TpTCP (Tcp src dst seq ack off flags win chksum urgent payload)
-      | TpICMP icmp => TpICMP icmp
-      | TpUnparsable proto payload => TpUnparsable proto payload
-    end.
-
-  Definition nw_setTpSrc (typ : dlTyp) (nwPkt : nw typ) tpSrc : nw typ :=
-    match nwPkt in nw typ return nw typ with
-      | NwIP (IP vhl tos len ident flags frag ttl proto chksum src dst tp) =>
-        NwIP (@IP vhl tos len ident flags frag ttl proto chksum src dst 
-                  (tp_setTpSrc tp tpSrc))
-      | NwARP arp => NwARP arp
-      | NwUnparsable typ b => NwUnparsable typ b
-    end.
-
-  Definition nw_setTpDst (typ : dlTyp) (nwPkt : nw typ) tpDst : nw typ :=
-    match nwPkt in nw typ return nw typ with
-      | NwIP (IP vhl tos len ident flags frag ttl proto chksum src dst tp) =>
-        NwIP (@IP vhl tos len ident flags frag ttl proto chksum src dst 
-                  (tp_setTpDst tp tpDst))
-      | NwARP arp => NwARP arp
-      | NwUnparsable typ b => NwUnparsable typ b
-    end.
-
-  Definition setTpSrc pk tpSrc :=
-    match pk with
-      | Packet dlSrc dlDst dlTyp dlVlan dlVlanPcp nw =>
-        @Packet dlSrc dlDst dlTyp dlVlan dlVlanPcp (nw_setTpSrc nw tpSrc)
-    end.
-
-  Definition setTpDst pk nwDst :=
-    match pk with
-      | Packet dlSrc dlDst dlTyp dlVlan dlVlanPcp nw =>
-        @Packet dlSrc dlDst dlTyp dlVlan dlVlanPcp (nw_setTpDst nw nwDst)
-    end.
-
-End Setters.
+*)
 
